\section{Proofs}
    \subsection{Proof that a group homomorphism maps $e$ to $e'$} \label{app:proof_hom_id}
        In this proof, we will prove that, given a group homomorphism $h$ between two groups $G$ and $G'$, that
        \begin{equation}
            h(e) = e' \thinspace ,
        \end{equation}
        in which $e$ is the idendity of $G$ and $e'$ is the identity of $G'$. \\

        We start off with
        \begin{align}
            h(e) &= h(e \cdot e)        && \text{$e$ is the identity element for $G$} \\
            &= h(e) \cdot' h(e)         && \text{$h$ is a group automorphism}
        \end{align}

        Next, since $G'$ is a group, we can multiply (via group multiplication in $G'$) both sides on the left by $h(e)^{-1}$:
        \begin{align}
            h(e)^{-1} \cdot' h(e) &= h(e)^{-1} \cdot' h(e) \cdot' h(e)      && \text{$h(e)^{-1}$ is the inverse of $h(e)$} \\
            e' &= e' \cdot' h(e)                                            && \text{$e'$ is the identity element in $G'$} \\
            e' &= h(e) \qed
        \end{align}

    \subsection{Proof that $h(a^{-1}) = h(a)^{-1}$} \label{app:proof_hom_inv}
        In this proof, we prove that, for a group homomorphism $h$ between two groups $G$ and $G'$, that
        \begin{equation}
            \forall a \in G: h(a^{-1}) = h(a)^{-1} \thinspace .
        \end{equation}

        Since $G$ is a group, we can start with
        \begin{align}
            \forall a \in G: h(a \cdot a^{-1}) &= h(e)      && \text{$a^{-1}$ is the inverse of $a$} \\
            &= h(a) \cdot' h(a^{-1})                        && \text{$h$ is a group homomorphism} \label{eq:hom_inv_1}
        \end{align}

        Furthermore, we know that
        \begin{align}
            \forall a \in G: e' &= h(a) \cdot' h(a)^{-1}    && \text{$h(a)^{-1}$ is the inverse of $h(a)$} \label{eq:hom_inv_2} \\
            &= h(e)                                         && \text{identity elements are mapped onto each other}
        \end{align}

        By combining equations (\ref{eq:hom_inv_1}) and (\ref{eq:hom_inv_2}), we find
        \begin{align}
            \forall a \in G: h(a) \cdot' h(a^{-1}) &= h(a) \cdot' h(a)^{-1}     && \text{multiply by $h(a)^{-1}$ on the left} \\
            \iff h(a^{-1}) &= h(a)^{-1} \qed
        \end{align}
